examples/box/Add01proof.v
@@ -1,0 +1,454 @@
+Require Import Mem0 Mem1 SimModSem Hoare.
+Require Import Coqlib.
+Require Import ITreelib.
+Require Import Universe.
+Require Import Skeleton.
+Require Import PCM.
+Require Import ModSem Behavior.
+Require Import Relation_Definitions.
+Require Import Add0 Add1 BoxHeader.
+
+(*** TODO: export these in Coqlib or Universe ***)
+Require Import Relation_Operators.
+Require Import RelationPairs.
+From ITree Require Import
+     Events.MapDefault.
+From ExtLib Require Import
+     Core.RelDec
+     Structures.Maps
+     Data.Map.FMapAList.
+
+Generalizable Variables E R A B C X Y.
+
+Set Implicit Arguments.
+
+Local Open Scope nat_scope.
+
+
+
+
+
+
+
+
+
+Definition tauK {E R}: R -> itree E R := fun r => tau;; Ret r.
+
+
+
+
+Lemma interp_vis:
+  forall (E F : Type -> Type) (R : Type) (f : forall T : Type, E T -> itree F T) (U : Type) (e : E U) (k : U -> itree E R),
+  interp f (Vis e k) = ` x : U <- f U e;; (tau;; interp f (k x))
+.
+Proof. i. f. eapply interp_vis. Qed.
+
+Lemma interp_ret: forall (E F : Type -> Type) (R : Type) (f : forall T : Type, E T -> itree F T) (x : R),
+    interp f (Ret x) = Ret x.
+Proof. i. f. eapply interp_ret. Qed.
+
+Lemma interp_tau: forall (E F : Type -> Type) (R : Type) (f : forall T : Type, E T -> itree F T) (t : itree E R),
+  interp f (tau;; t) = (tau;; interp f t).
+Proof. i. f. eapply interp_tau. Qed.
+
+Lemma interp_trigger:
+  forall (E F : Type -> Type) (R : Type) (f : forall T : Type, E T -> itree F T) (e : E R),
+  interp f (ITree.trigger e) = x <- (f R e);; tau;; Ret x
+  (* (f R e) >>= tauK *)
+.
+Proof.
+  i. unfold ITree.trigger.
+  rewrite interp_vis. f_equiv. apply func_ext. i. unfold tauK. repeat f_equiv. rewrite interp_ret. ss.
+Qed.
+
+Hint Unfold tauK.
+
+Lemma interp_bind :
+forall {E F : Type -> Type} {R S : Type} (f : forall T : Type, E T -> itree F T) 
+  (t : itree E R) (k : R -> itree E S),
+interp f (` x : _ <- t;; k x) = ` r : R <- interp f t;; interp f (k r).
+Proof. i. f. apply interp_bind. Qed.
+
+
+
+(*** black + delta --> new_black ***)
+Definition add_delta_to_black `{M: URA.t} (b: URA.auth_t) (w: URA.auth_t): URA.auth_t :=
+  match b, w with
+  | URA.excl e _, URA.frag f1 => URA.excl (URA.add e f1) URA.unit
+  | _, _ => URA.boom
+  end
+.
+
+
+
+
+
+
+
+Ltac go := try first[pfold; econs; [..|M]; (Mskip ss); et; check_safe; ii; left|
+                     pfold; econsr; [..|M]; (Mskip ss); et; check_safe; ii; left].
+Ltac force_l := pfold; econs; [..|M]; Mskip ss; et.
+Ltac force_r := pfold; econsr; [..|M]; Mskip ss; et.
+Section SIMMODSEM.
+
+  Context `{Σ: GRA.t}.
+  Context `{@GRA.inG boxRA Σ}.
+
+
+
+
+
+
+
+
+
+
+
+
+
+
+
+
+
+
+
+
+
+
+
+
+
+
+
+
+
+
+
+
+
+  Lemma interp_state_bind:
+  forall (E F : Type -> Type) (A B S : Type) (f : forall T : Type, E T -> S -> itree F (S * T)) (t : itree E A)
+    (k : A -> itree E B) (s : S),
+  interp_state f (` x : _ <- t;; k x) s = ` st : S * A <- interp_state f t s;; interp_state f (k (snd st)) (fst st)
+  .
+  Proof. i. f. apply interp_state_bind. Qed.
+
+  Lemma interp_state_vis:
+  forall (E F : Type -> Type) (S T U : Type) (e : E T) (k : T -> itree E U) (h : forall T0 : Type, E T0 -> stateT S (itree F) T0)
+    (s : S), interp_state h (Vis e k) s = ` sx : S * T <- h T e s;; (tau;; interp_state h (k (snd sx)) (fst sx))
+  .
+  Proof.
+    i. f. apply interp_state_vis.
+  Qed.
+
+  Lemma interp_state_tau :
+    forall (E F : Type -> Type) (S T : Type) (t : itree E T) (h : forall T0 : Type, E T0 -> stateT S (itree F) T0) (s : S),
+      interp_state h (tau;; t) s = (tau;; interp_state h t s)
+  .
+  Proof.
+    i. f. apply interp_state_tau.
+  Qed.
+
+  Lemma interp_state_ret:
+  forall (E F : Type -> Type) (R S : Type) (f : forall T : Type, E T -> S -> itree F (S * T)) (s : S) (r : R),
+  interp_state f (Ret r) s = Ret (s, r)
+  .
+  Proof.
+    i. f. apply interp_state_ret.
+  Qed.
+
+  Lemma unfold_interp:
+    forall (E F : Type -> Type) (R : Type) (f : forall T : Type, E T -> itree F T) (t : itree E R),
+      interp f t = _interp f (observe t)
+  .
+  Proof.
+    i. f. apply unfold_interp.
+  Qed.
+
+  Definition my_interp A (prog: callE ~> itree Es) (itr0: itree Es A) (st0: ModSem.r_state) :=
+    ModSem.interp_rE (interp_mrec prog itr0) st0
+  .
+
+  Ltac grind := repeat (f_equiv; try apply func_ext; ii; try (des_ifs; check_safe)).
+
+  Lemma my_interp_bind
+        (prog: callE ~> itree Es)
+        A B
+        (itr: itree Es A) (ktr: A -> itree Es B)
+        st0
+    :
+      my_interp prog (v <- itr ;; ktr v) st0 =
+      '(st1, v) <- my_interp prog (itr) st0 ;; my_interp prog (ktr v) st1
+  .
+  Proof.
+    unfold my_interp.
+    unfold ModSem.interp_rE.
+    rewrite interp_mrec_bind.
+    rewrite interp_state_bind.
+    grind.
+  Qed.
+
+  Lemma my_interp_tau
+        (prog: callE ~> itree Es)
+        A
+        (itr: itree Es A)
+        st0
+    :
+      my_interp prog (tau;; itr) st0 = tau;; my_interp prog itr st0
+  .
+  Proof.
+    unfold my_interp.
+    unfold ModSem.interp_rE.
+    rewrite unfold_interp_mrec. ss.
+    rewrite interp_state_tau.
+    grind.
+  Qed.
+
+  Lemma my_interp_ret
+        T
+        prog st0 (v: T)
+    :
+      my_interp prog (Ret v) st0 = Ret (st0, v)
+  .
+  Proof.
+    unfold my_interp. unfold ModSem.interp_rE.
+    rewrite unfold_interp_mrec. ss.
+    rewrite interp_state_ret. ss.
+  Qed.
+
+  Lemma interp_mrec_hit:
+    forall (D E : Type -> Type) (ctx : forall T : Type, D T -> itree (D +' E) T) (U : Type) (a : D U),
+      interp_mrec ctx (trigger a) = (tau;; interp_mrec ctx (ctx _ a))
+  .
+  Proof.
+    i. rewrite unfold_interp_mrec. ss.
+    unfold resum, ReSum_id, id_, Id_IFun. rewrite bind_ret_r. ss.
+  Qed.
+
+
+  Definition idK {E R}: R -> itree E R := fun r => Ret r.
+  Hint Unfold idK.
+
+  Lemma idK_spec E R (i0: itree E R): i0 = i0 >>= idK. Proof. unfold idK. irw. refl. Qed.
+
+  (*** TODO: I don't want "F" here, but it is technically needed. Report it to itree people? ***)
+  Lemma interp_mrec_miss:
+    (* forall (D E F: Type -> Type) `{F -< E} (ctx : forall T : Type, D T -> itree (D +' E) T) (U : Type) (a : F U), *)
+    forall (D E F: Type -> Type) `{F -< E} (ctx : forall T : Type, D T -> itree (D +' E) T) (U : Type) (a : F U),
+      interp_mrec ctx (trigger a) = x <- (trigger a);; tau;; Ret x
+      (* (trigger a) >>= tauK *)
+  .
+  Proof.
+    i. rewrite unfold_interp_mrec. cbn.
+    unfold trigger. irw.
+    grind. irw. ss.
+  Qed.
+
+  (*** TODO: interp_trigger_eqit does not exist. report to itree people? ***)
+  Lemma interp_state_trigger:
+  forall (E F : Type -> Type) (R S : Type) (e : E R) (f : forall T : Type, E T -> stateT S (itree F) T) (s : S),
+  interp_state f (ITree.trigger e) s = ` x : S * R <- f R e s;; (tau;; Ret x)
+  .
+  Proof. i. f. apply interp_state_trigger_eqit. Qed.
+
+  Lemma my_interp_callE
+        p st0
+        (* (e: Es Σ) *)
+        (e: callE val)
+    :
+      my_interp p (trigger e) st0 = tau;; (my_interp p (p val e) st0)
+  .
+  Proof.
+    unfold my_interp. unfold ModSem.interp_rE. rewrite interp_mrec_hit. cbn.
+    rewrite interp_state_tau. grind.
+  Qed.
+
+  Lemma my_interp_rE
+        p st0
+        (* (e: Es Σ) *)
+        T
+        (e: rE T)
+    :
+      my_interp p (trigger e) st0 =
+      '(st1, r) <- ModSem.handle_rE e st0;;
+      tau;; tau;;
+      Ret (st1, r)
+      (* interp_state (case_ ModSem.handle_rE pure_state) (tau;; Ret r) st1 *)
+  .
+  Proof.
+    unfold my_interp. unfold ModSem.interp_rE.
+    (* rewrite unfold_interp_mrec. cbn. *)
+    unfold Es.
+    rewrite interp_mrec_miss with (D:=callE) (E:=rE +' eventE) (F:=rE) (a:=e).
+    rewrite interp_state_bind.
+    rewrite interp_state_trigger. irw. grind. irw. grind.
+    rewrite interp_state_tau. grind.
+    rewrite interp_state_ret. ss.
+  Qed.
+
+  Lemma my_interp_eventE
+        p st0
+        (* (e: Es Σ) *)
+        T
+        (e: eventE T)
+    :
+      my_interp p (trigger e) st0 = r <- trigger e;; tau;; tau;; Ret (st0, r)
+  .
+  Proof.
+    unfold my_interp. unfold ModSem.interp_rE.
+    (* rewrite unfold_interp_mrec. cbn. *)
+    unfold Es.
+    rewrite interp_mrec_miss with (D:=callE) (E:=rE +' eventE) (F:=eventE) (a:=e).
+    rewrite interp_state_bind.
+    rewrite interp_state_trigger. irw. unfold pure_state.
+    unfold resum, ReSum_id, id_, Id_IFun.
+    irw. grind. irw. grind.
+    rewrite interp_state_tau. grind.
+    rewrite interp_state_ret. ss.
+  Qed.
+
+  Lemma my_interp_triggerUB
+        (prog: callE ~> itree Es)
+        st0
+        A
+    :
+      (my_interp prog (triggerUB) st0: itree eventE (_ * A)) = triggerUB
+  .
+  Proof.
+    unfold triggerUB. rewrite my_interp_bind. rewrite my_interp_eventE.
+    irw. grind.
+  Qed.
+
+  Lemma my_interp_triggerNB
+        (prog: callE ~> itree Es)
+        st0
+        A
+    :
+      (my_interp prog (triggerNB) st0: itree eventE (_ * A)) = triggerNB
+  .
+  Proof.
+    unfold triggerNB. rewrite my_interp_bind. rewrite my_interp_eventE.
+    irw. grind.
+  Qed.
+
+  Ltac igo := repeat (try rewrite bind_bind; try rewrite bind_ret_l; try rewrite bind_ret_r; try rewrite bind_tau;
+                      try rewrite interp_vis;
+                      try rewrite interp_ret;
+                      try rewrite interp_tau;
+                      (* try rewrite interp_trigger *)
+                      try rewrite interp_bind
+                     ).
+
+
+
+
+
+
+
+
+
+
+
+
+
+
+
+
+
+
+
+  Let W: Type := (alist mname Σ) * (alist mname Σ).
+
+  Let wf: W -> Prop :=
+    fun '(mrs_src0, mrs_tgt0) =>
+      exists mr_src mr_tgt,
+        (<<SRC: alist_find Dec_RelDec "Add" mrs_src0 = Some mr_src>>) /\
+        (<<TGT: alist_find Dec_RelDec "Add" mrs_tgt0 = Some mr_tgt>>)
+  .
+
+  Local Opaque GRA.to_URA.
+  Infix "⋅" := URA.add (at level 50, left associativity).
+  Notation "(⋅)" := URA.add (only parsing).
+
+  Local Opaque AddStb BoxStb.
+  Local Opaque string_dec.
+  Theorem correct: ModSemPair.sim Add1.AddSem Add0.AddSem.
+  Proof.
+    econstructor 1 with (wf:=wf) (le:=top2); et; swap 2 3.
+    { typeclasses eauto. }
+    { ss. esplits; ss; et. }
+    econs; ss.
+    { split; ss. ii; clarify. rename y into varg. eexists 100%nat. ss. des; clarify.
+      unfold alist_add, alist_remove; ss.
+      unfold addF.
+      repeat (go; igo; ss).
+      unfold assume, guarantee.
+      repeat (go; igo; ss).
+      des; clarify.
+      rewrite ! URA.unit_idl.
+      (* unfold unwrapU. des_ifs. igo. *)
+      unfold addBody.
+      unfold body_to_tgt. unfold interp_hCallE_tgt. igo. rewrite interp_trigger. cbn. des_ifs.
+      Local Transparent BoxStb AddStb.
+      cbn in Heq.
+      Local Opaque BoxStb AddStb.
+      des_ifs. cbn in *. clear_tac.
+      repeat (go; igo; ss).
+      rewrite URA.unit_idl in WF.
+      unfold HoareCall.
+      repeat (go; igo; ss).
+
+
+      force_l. eexists (mr_src, client x). left.
+      repeat (go; igo; ss).
+      force_l. left.
+      force_l. eexists. left.
+      repeat (go; igo; ss).
+      force_l. { rewrite URA.unit_idl; try refl. } left.
+      force_l. eexists. left.
+      repeat (go; igo; ss).
+      unfold assume, guarantee.
+      repeat (go; igo; ss).
+      force_l. unshelve eexists; et. left.
+      pfold; econs; et.
+      { ss. esplits; et. }
+      ii. exists 100%nat. left.
+      repeat (go; igo; ss). des.
+      repeat (go; igo; ss). des. clarify.
+      repeat (go; igo; ss).
+      rewrite interp_trigger.
+      repeat (go; igo; ss). cbn. des_ifs.
+      Local Transparent BoxStb AddStb.
+      cbn in Heq.
+      Local Opaque BoxStb AddStb.
+      des_ifs. cbn in *.
+      unfold HoareCall.
+      repeat (go; igo; ss).
+      force_l. eexists (mr_src0, client x). left.
+      repeat (go; igo; ss).
+      force_l. { rewrite URA.unit_idl. eapply URA.updatable_add; try refl. } left.
+      force_l. eexists (client x). left.
+      repeat (go; igo; ss).
+      force_l. { rewrite URA.unit_idl; ss. } left.
+      force_l. exists ((x+1)%Z). left.
+      repeat (go; igo; ss).
+      unfold assume, guarantee.
+      repeat (go; igo; ss).
+      force_l. unshelve eexists; et. left.
+      rewrite idK_spec with (i0:=trigger (Call "set" [Vint (x+1)])). unfold idK at 1. rewrite bind_bind.
+      pfold. econs; ss; et.
+      ii. des. eexists 100%nat. left.
+      repeat (go; igo; ss). clarify.
+      force_l. eexists (mr_src1, client (x+1)). left.
+      force_l. { rewrite URA.unit_idl. eapply URA.updatable_add; try refl. } left.
+      force_l. eexists (client (x+1)). left.
+      repeat (go; igo; ss).
+      force_l. unshelve eexists; et. left.
+      force_l. { rewrite URA.unit_idl; ss. } left.
+      pfold. econs; ss; et.
+    }
+  Qed.
+
+End SIMMODSEM.
+
+
