examples/box/Add1.v
@@ -1,0 +1,49 @@
+Require Import Coqlib.
+Require Import ITreelib.
+Require Import Universe.
+Require Import STS.
+Require Import Behavior.
+Require Import ModSem.
+Require Import Skeleton.
+Require Import PCM.
+Require Import Hoare.
+
+Require Import BoxHeader.
+
+Generalizable Variables E R A B C X Y Σ.
+
+Set Implicit Arguments.
+Set Typeclasses Depth 4.
+
+
+
+
+Section PROOF.
+  Context `{@GRA.inG boxRA Σ}.
+  (* Let GURA: URA.t := GRA.to_URA Σ. *)
+  (* Local Existing Instance GURA. *)
+
+  Definition addBody (varg: list val): itree (hCallE +' eventE) val :=
+    x <- trigger (hCall "get" []);;
+    x_plus_one <- vadd x (Vint 1%Z)?;;
+    trigger (hCall "set" [x_plus_one])
+  .
+
+  Definition AddFtb: list (fname * (list val -> itree (hCallE +' eventE) val)) :=
+    zip pair ["add"] [addBody]
+  .
+
+  Definition AddSem: ModSem.t :=
+    {|
+      ModSem.fnsems := List.map (fun '(fn, body) => (fn, fun_to_tgt (BoxStb++AddStb) fn body)) AddFtb;
+      ModSem.initial_mrs := [("Add", URA.unit)];
+    |}
+  .
+
+  Definition Add: Mod.t := {|
+    Mod.get_modsem := fun _ => AddSem; (*** TODO: we need proper handling of function pointers ***)
+    Mod.sk := Sk.unit;
+  |}
+  .
+
+End PROOF.
